x64: port device-untyped from ARM

proof/invariant-abstract/X64/ArchInvariants_AI.thy
@@ -37,7 +37,7 @@ lemma arch_cap_fun_lift_expand[simp]:
   "(arch_cap_fun_lift (\<lambda> ac. case ac of
                                 ASIDPoolCap obj_ref asid \<Rightarrow> P_ASIDPoolCap obj_ref asid
                               | ASIDControlCap \<Rightarrow> P_ASIDControlCap
-                              | PageCap obj_ref rights maptyp sz vr \<Rightarrow> P_PageCap obj_ref rights maptyp sz vr
+                              | PageCap dev obj_ref rights maptyp sz vr \<Rightarrow> P_PageCap dev obj_ref rights maptyp sz vr
                               | PageTableCap obj_ref vr \<Rightarrow> P_PageTableCap obj_ref vr
                               | PageDirectoryCap obj_ref vr \<Rightarrow> P_PageDirectoryCap obj_ref vr
                               | PDPointerTableCap obj_ref vr \<Rightarrow> P_PDPointerTableCap obj_ref vr
@@ -51,7 +51,7 @@ lemma arch_cap_fun_lift_expand[simp]:
    (case c of
       ArchObjectCap (ASIDPoolCap obj_ref asid) \<Rightarrow> P_ASIDPoolCap obj_ref asid
     | ArchObjectCap (ASIDControlCap) \<Rightarrow> P_ASIDControlCap
-    | ArchObjectCap (PageCap obj_ref rights maptyp sz vr) \<Rightarrow> P_PageCap obj_ref rights maptyp sz vr
+    | ArchObjectCap (PageCap dev obj_ref rights maptyp sz vr) \<Rightarrow> P_PageCap dev obj_ref rights maptyp sz vr
     | ArchObjectCap (PageTableCap obj_ref vr) \<Rightarrow> P_PageTableCap obj_ref vr
     | ArchObjectCap (PageDirectoryCap obj_ref asid) \<Rightarrow> P_PageDirectoryCap obj_ref asid
     | ArchObjectCap (PDPointerTableCap obj_ref vr) \<Rightarrow> P_PDPointerTableCap obj_ref vr
@@ -70,7 +70,7 @@ lemma arch_obj_fun_lift_expand[simp]:
                                 ASIDPool pool \<Rightarrow> P_ASIDPool pool
                               | PageTable pt \<Rightarrow> P_PageTable pt
                               | PageDirectory pd \<Rightarrow> P_PageDirectory pd
-                              | DataPage s \<Rightarrow> P_DataPage s
+                              | DataPage dev s \<Rightarrow> P_DataPage dev s
                               | PDPointerTable pdpt \<Rightarrow> P_PDPT pdpt
                               | PageMapL4 pml \<Rightarrow> P_PML4 pml)
                       F) = (\<lambda>ko. 
@@ -78,7 +78,7 @@ lemma arch_obj_fun_lift_expand[simp]:
       ArchObj (ASIDPool pool) \<Rightarrow> P_ASIDPool pool
     | ArchObj (PageTable pt) \<Rightarrow> P_PageTable pt
     | ArchObj (PageDirectory pd) \<Rightarrow> P_PageDirectory pd
-    | ArchObj (DataPage s) \<Rightarrow> P_DataPage s
+    | ArchObj (DataPage dev s) \<Rightarrow> P_DataPage dev s
     | ArchObj (PDPointerTable pdpt) \<Rightarrow> P_PDPT pdpt
     | ArchObj (PageMapL4 pml) \<Rightarrow> P_PML4 pml
     | _ \<Rightarrow> F))"
@@ -107,7 +107,7 @@ where
    case ac of
      ASIDPoolCap r as
        \<Rightarrow> is_aligned as asid_low_bits \<and> as \<le> 2^asid_bits - 1
-   | PageCap r rghts maptyp sz mapdata \<Rightarrow> rghts \<in> valid_vm_rights \<and>
+   | PageCap dev r rghts maptyp sz mapdata \<Rightarrow> rghts \<in> valid_vm_rights \<and>
      case_option True (wellformed_mapdata sz) mapdata
    | PageTableCap r (Some mapdata) \<Rightarrow>
      wellformed_mapdata X64LargePage mapdata
@@ -123,6 +123,35 @@ where
 lemmas wellformed_acap_simps =
   wellformed_mapdata_def wellformed_acap_def[split_simps arch_cap.split]
 
+definition
+  "in_device_frame p \<equiv> \<lambda>s.
+   \<exists>sz. typ_at (AArch (ADeviceData sz)) (p && ~~ mask (pageBitsForSize sz)) s"
+
+definition
+  "user_mem s \<equiv> \<lambda>p.
+  if (in_user_frame p s)
+  then Some (underlying_memory (machine_state s) p)
+  else None"
+
+definition
+  "device_mem s \<equiv> \<lambda>p.
+  if (in_device_frame p s)
+  then Some p
+  else None"
+
+abbreviation "device_region s \<equiv> dom (device_state (machine_state s))"
+
+lemma typ_at_pg_user:
+  "typ_at (AArch (AUserData sz)) buf s = ko_at (ArchObj (DataPage False sz)) buf s"
+  unfolding obj_at_def
+  by (auto simp: a_type_def split: Structures_A.kernel_object.split_asm arch_kernel_obj.split_asm split_if_asm)
+
+lemma typ_at_pg_device:
+  "typ_at (AArch (ADeviceData sz)) buf s = ko_at (ArchObj (DataPage True sz)) buf s"
+  unfolding obj_at_def
+  by (auto simp: a_type_def split: Structures_A.kernel_object.split_asm arch_kernel_obj.split_asm split_if_asm)
+
+lemmas typ_at_pg = typ_at_pg_user typ_at_pg_device
 
 (* this time with typ_at. might lead to confusion, but this is how
    the rest should have been defined.. *)
@@ -157,7 +186,9 @@ where
     ASIDPoolCap r as \<Rightarrow> typ_at (AArch AASIDPool) r s
   | ASIDControlCap \<Rightarrow> True
   | IOPortCap first_port last_port \<Rightarrow> True
-  | PageCap r rghts maptyp sz mapdata \<Rightarrow> typ_at (AArch (AIntData sz)) r s
+  | PageCap dev r rghts maptyp sz mapdata \<Rightarrow>
+      if dev then typ_at (AArch (ADeviceData sz)) r s
+             else typ_at (AArch (AUserData sz)) r s
   | PageTableCap r mapdata \<Rightarrow> typ_at (AArch APageTable) r s
   | PageDirectoryCap r mapdata\<Rightarrow> typ_at (AArch APageDirectory) r s
   | PDPointerTableCap r mapdata \<Rightarrow> typ_at (AArch APDPointerTable) r s
@@ -175,8 +206,10 @@ where
            \<and> as \<le> 2^asid_bits - 1
   | ASIDControlCap \<Rightarrow> True
   | IOPortCap first_port last_port \<Rightarrow> True
-  | PageCap r rghts maptyp sz mapdata \<Rightarrow>
-    typ_at (AArch (AIntData sz)) r s \<and> rghts \<in> valid_vm_rights \<and>
+  | PageCap dev r rghts maptyp sz mapdata \<Rightarrow>
+    (if dev then (typ_at (AArch (ADeviceData sz)) r s)
+            else (typ_at (AArch (AUserData sz)) r s)) \<and>
+    (rghts \<in> valid_vm_rights) \<and>
     (case mapdata of None \<Rightarrow> True | Some (asid, ref) \<Rightarrow> 0 < asid \<and> asid \<le> 2^asid_bits - 1
                                              \<and> vmsz_aligned ref sz \<and> ref < kernel_base)
   | PageTableCap r mapdata \<Rightarrow>
@@ -202,12 +235,27 @@ where
 lemmas valid_arch_cap_simps =
   valid_arch_cap_def[split_simps arch_cap.split]
 
+definition
+  "is_nondevice_page_cap_arch \<equiv> \<lambda>cap. case cap of (PageCap False _ _ _ _ _) \<Rightarrow>  True
+                                                 | _ \<Rightarrow> False"
+
+declare is_nondevice_page_cap_arch_def [simp]
+
+definition
+  "is_nondevice_page_cap \<equiv> \<lambda>c. arch_cap_fun_lift is_nondevice_page_cap_arch False c"
+
+lemma is_nondevice_page_cap:
+  "is_nondevice_page_cap c = (\<exists> p q r s t. c = ArchObjectCap (PageCap False p q r s t))"
+  by (auto simp: is_nondevice_page_cap_def split: cap.splits arch_cap.splits)
+
+lemmas is_nondevice_page_cap_simps = is_nondevice_page_cap
+
 primrec
   acap_class :: "arch_cap \<Rightarrow> capclass"
 where
   "acap_class (ASIDPoolCap x y)       = PhysicalClass"
 | "acap_class (ASIDControlCap)        = ASIDMasterClass"
-| "acap_class (PageCap x y m sz z)    = PhysicalClass"
+| "acap_class (PageCap d x y m sz z)  = PhysicalClass"
 | "acap_class (PageTableCap x y)      = PhysicalClass"
 | "acap_class (PageDirectoryCap x y)  = PhysicalClass"
 | "acap_class (PDPointerTableCap x y) = PhysicalClass"
@@ -219,31 +267,36 @@ definition
 where
   "valid_ipc_buffer_cap_arch ac bufptr \<equiv>
          case ac of
-              (PageCap ref rghts maptyp sz mapdata) \<Rightarrow>
+              (PageCap False ref rghts maptyp sz mapdata) \<Rightarrow>
                    is_aligned bufptr msg_align_bits
-            | _ \<Rightarrow> True"
+            | _ \<Rightarrow> False"
 
 declare valid_ipc_buffer_cap_arch_def[simp]
 
 definition
-  "valid_ipc_buffer_cap c bufptr \<equiv> 
-     arch_cap_fun_lift (\<lambda>ac. valid_ipc_buffer_cap_arch ac bufptr) True c"
+  "valid_ipc_buffer_cap c bufptr \<equiv>
+    case c of
+      NullCap \<Rightarrow> True
+    | ArchObjectCap acap \<Rightarrow> valid_ipc_buffer_cap_arch acap bufptr
+    | _ \<Rightarrow> False"
+
+definition "data_at \<equiv>
+  \<lambda>sz p s. typ_at (AArch (AUserData sz)) p s
+         \<or> typ_at (AArch (ADeviceData sz)) p s"
 
 primrec
   valid_pte :: "pte \<Rightarrow> 'z::state_ext state \<Rightarrow> bool"
 where
   "valid_pte (InvalidPTE) = \<top>"
 | "valid_pte (SmallPagePTE ptr x y) =
-   (\<lambda>s. vmsz_aligned ptr X64SmallPage \<and>
-        typ_at (AArch (AIntData X64SmallPage)) (ptrFromPAddr ptr) s)"
+   (\<lambda>s. vmsz_aligned ptr X64SmallPage \<and> data_at X64SmallPage (ptrFromPAddr ptr) s)"
 
 primrec
   valid_pde :: "pde \<Rightarrow> 'z::state_ext state \<Rightarrow> bool"
 where
   "valid_pde (InvalidPDE) = \<top>"
 | "valid_pde (LargePagePDE ptr x y) =
-   (\<lambda>s. vmsz_aligned ptr X64LargePage \<and>
-        typ_at (AArch (AIntData X64LargePage)) (ptrFromPAddr ptr) s)"
+   (\<lambda>s. vmsz_aligned ptr X64LargePage \<and> data_at X64LargePage (ptrFromPAddr ptr) s)"
 | "valid_pde (PageTablePDE ptr x z) =
    (typ_at (AArch APageTable) (ptrFromPAddr ptr))"
 
@@ -252,8 +305,7 @@ primrec
 where
   "valid_pdpte (InvalidPDPTE) = \<top>"
 | "valid_pdpte (HugePagePDPTE ptr x y) =
-   (\<lambda>s. vmsz_aligned ptr X64HugePage \<and>
-        typ_at (AArch (AIntData X64HugePage)) (ptrFromPAddr ptr) s)"
+   (\<lambda>s. vmsz_aligned ptr X64HugePage \<and> data_at X64HugePage (ptrFromPAddr ptr) s)"
 | "valid_pdpte (PageDirectoryPDPTE ptr x z) =
    (typ_at (AArch APageDirectory) (ptrFromPAddr ptr))"
 
@@ -281,7 +333,7 @@ where
 | "valid_arch_obj (PDPointerTable pdpt) = (\<lambda>s. \<forall>x. valid_pdpte (pdpt x) s)"
 | "valid_arch_obj (PageDirectory pd) = (\<lambda>s. \<forall>x. valid_pde (pd x) s)"
 | "valid_arch_obj (PageTable pt) = (\<lambda>s. \<forall>x. valid_pte (pt x) s)"
-| "valid_arch_obj (DataPage sz) = \<top>"
+| "valid_arch_obj (DataPage dev sz) = \<top>"
 
 
 (* FIXME x64: check hardware to see if any bits are forbidden *)
@@ -827,7 +879,7 @@ definition
   valid_arch_state :: "'z::state_ext state \<Rightarrow> bool"
 where
   "valid_arch_state \<equiv> \<lambda>s.
-  typ_at (AArch (AIntData X64SmallPage)) (x64_globals_frame (arch_state s)) s \<and>
+  typ_at (AArch (AUserData X64SmallPage)) (x64_globals_frame (arch_state s)) s \<and>
   valid_asid_table (x64_asid_table (arch_state s)) s \<and>
   page_map_l4_at (x64_global_pml4 (arch_state s)) s \<and>
   valid_global_pts s \<and> valid_global_pds s \<and> valid_global_pdpts s"
@@ -856,20 +908,20 @@ where
            VSRef ((vptr >> 39) && mask 9) (Some APageMapL4),
            VSRef (asid && mask asid_low_bits) (Some AASIDPool),
            VSRef (ucast (asid_high_bits_of asid)) None]
- | PageCap word rights typ X64SmallPage (Some (asid, vptr)) \<Rightarrow>
+ | PageCap dev word rights typ X64SmallPage (Some (asid, vptr)) \<Rightarrow>
      Some [VSRef ((vptr >> 12) && mask 9) (Some APageTable),
            VSRef ((vptr >> 21) && mask 9) (Some APageDirectory),
            VSRef ((vptr >> 30) && mask 9) (Some APDPointerTable),
            VSRef ((vptr >> 39) && mask 9) (Some APageMapL4),
            VSRef (asid && mask asid_low_bits) (Some AASIDPool),
            VSRef (ucast (asid_high_bits_of asid)) None]
- | PageCap word rights typ X64LargePage  (Some (asid, vptr)) \<Rightarrow>
+ | PageCap dev word rights typ X64LargePage  (Some (asid, vptr)) \<Rightarrow>
      Some [VSRef ((vptr >> 21) && mask 9) (Some APageDirectory),
            VSRef ((vptr >> 30) && mask 9) (Some APDPointerTable),
            VSRef ((vptr >> 39) && mask 9) (Some APageMapL4),
            VSRef (asid && mask asid_low_bits) (Some AASIDPool),
            VSRef (ucast (asid_high_bits_of asid)) None]
- | PageCap word rights typ X64HugePage (Some (asid, vptr)) \<Rightarrow>
+ | PageCap dev word rights typ X64HugePage (Some (asid, vptr)) \<Rightarrow>
      Some [VSRef ((vptr >> 30) && mask 9) (Some APDPointerTable),
            VSRef ((vptr >> 39) && mask 9) (Some APageMapL4),
            VSRef (asid && mask asid_low_bits) (Some AASIDPool),
@@ -882,10 +934,10 @@ definition
   "vs_cap_ref cap \<equiv> arch_cap_fun_lift vs_cap_ref_arch None cap"
 
 definition
-  "is_pg_cap cap \<equiv> \<exists>p R tp sz m. cap = ArchObjectCap (PageCap p R tp sz m)"
+  "is_pg_cap cap \<equiv> \<exists>dev p R tp sz m. cap = ArchObjectCap (PageCap dev p R tp sz m)"
 
 definition
-  "is_page_cap cap \<equiv> \<exists>p R tp sz m. cap = PageCap p R tp sz m"
+  "is_page_cap cap \<equiv> \<exists>d p R tp sz m. cap = PageCap d p R tp sz m"
 
 definition
   "is_pml4_cap c \<equiv>
@@ -907,17 +959,15 @@ lemmas is_vspace_table_cap_defs = is_pt_cap_def is_pd_cap_def is_pdpt_cap_def is
 abbreviation
   "is_vspace_table_cap c \<equiv> is_pt_cap c \<or> is_pd_cap c \<or> is_pdpt_cap c \<or> is_pml4_cap c"
 
-lemma is_arch_cap_simps:
-  "is_pg_cap cap   = (\<exists>p R ty sz m. cap = (ArchObjectCap (PageCap p R ty sz m)))"
-  "is_pd_cap cap   = (\<exists>p asid. cap = (ArchObjectCap (PageDirectoryCap p asid)))"
-  "is_pt_cap cap   = (\<exists>p asid. cap = (ArchObjectCap (PageTableCap p asid)))"
-  "is_pdpt_cap cap = (\<exists>p asid. cap = (ArchObjectCap (PDPointerTableCap p asid)))"
-  "is_pml4_cap cap = (\<exists>p asid. cap = (ArchObjectCap (PML4Cap p asid)))"
-  by (auto simp add: is_pg_cap_def is_pd_cap_def is_pt_cap_def is_pdpt_cap_def is_pml4_cap_def)
+
+lemmas is_arch_cap_simps [simplified atomize_eq] =
+  is_pg_cap_def is_pd_cap_def is_pt_cap_def is_pdpt_cap_def is_pml4_cap_def
+  is_nondevice_page_cap
+
 
 definition
   "cap_asid_arch cap \<equiv> case cap of
-    PageCap _ _ _ _ (Some (asid, _)) \<Rightarrow> Some asid
+    PageCap _ _ _ _ _ (Some (asid, _)) \<Rightarrow> Some asid
   | PageTableCap _ (Some (asid, _)) \<Rightarrow> Some asid
   | PageDirectoryCap _ (Some (asid, _)) \<Rightarrow> Some asid
   | PDPointerTableCap _ (Some (asid, _)) \<Rightarrow> Some asid
@@ -1049,7 +1099,8 @@ definition
 where
  "arch_obj_bits_type T' \<equiv> (case T' of
     AASIDPool \<Rightarrow> arch_kobj_size (ASIDPool undefined)
-  | AIntData sz \<Rightarrow> arch_kobj_size (DataPage sz)
+  | ADeviceData sz \<Rightarrow> arch_kobj_size (DataPage True sz)
+  | AUserData sz \<Rightarrow> arch_kobj_size (DataPage False sz)
   | APageDirectory \<Rightarrow> arch_kobj_size (PageDirectory undefined)
   | APageTable \<Rightarrow> arch_kobj_size (PageTable undefined)
   | APDPointerTable \<Rightarrow> arch_kobj_size (PDPointerTable undefined)
@@ -1214,28 +1265,28 @@ lemma valid_arch_cap_typ:
   shows      "\<lbrace>\<lambda>s. valid_arch_cap c s\<rbrace> f \<lbrace>\<lambda>rv s. valid_arch_cap c s\<rbrace>"
   apply (simp add: valid_arch_cap_def)
   apply (case_tac c, simp_all)
-  by (wp P)
+  by (wp P hoare_vcg_ball_lift hoare_vcg_imp_lift hoare_vcg_conj_lift | clarsimp)+
 
 lemma valid_arch_obj_typ:
   assumes P: "\<And>p T. \<lbrace>\<lambda>s. (typ_at (AArch T) p s)\<rbrace> f \<lbrace>\<lambda>rv s.  (typ_at (AArch T) p s)\<rbrace>"
   shows      "\<lbrace>\<lambda>s. valid_arch_obj ob s\<rbrace> f \<lbrace>\<lambda>rv s. valid_arch_obj ob s\<rbrace>"
   apply (cases ob, simp_all)
-       apply (rule hoare_vcg_ball_lift [OF P])
+       apply (rule hoare_vcg_const_Ball_lift[OF P])
       apply (rule hoare_vcg_all_lift)
       apply (rename_tac "fun" x)
-      apply (case_tac "fun x"; simp; wp P)
-     apply (rule hoare_vcg_all_lift)
-     apply (rename_tac "fun" x)
-     apply (case_tac "fun x"; simp; wp P)
+      apply (case_tac "fun x", simp_all add: data_at_def hoare_vcg_prop P)
+     apply (wp hoare_vcg_disj_lift P)
     apply (rule hoare_vcg_all_lift)
     apply (rename_tac "fun" x)
-    apply (case_tac "fun x"; simp; wp P)
-   apply (rule hoare_vcg_ball_lift)
+    apply (case_tac "fun x", simp_all add: data_at_def hoare_vcg_prop P)
+    apply (wp hoare_vcg_disj_lift P)
+   apply (rule hoare_vcg_all_lift)
    apply (rename_tac "fun" x)
-   apply (case_tac "fun x";simp; wp P)
-  apply wp
+   apply (case_tac "fun x", simp_all add: data_at_def hoare_vcg_prop P)
+   apply (wp hoare_vcg_disj_lift hoare_vcg_const_Ball_lift P)
+  apply (rename_tac "fun" x)
+  apply (case_tac "fun x", simp_all add: hoare_vcg_prop P)
   done
-
 
 lemma atyp_at_eq_kheap_obj:
   "typ_at (AArch AASIDPool) p s \<longleftrightarrow> (\<exists>f. kheap s p = Some (ArchObj (ASIDPool f)))"
@@ -1243,7 +1294,8 @@ lemma atyp_at_eq_kheap_obj:
   "typ_at (AArch APageDirectory) p s \<longleftrightarrow> (\<exists>pd. kheap s p = Some (ArchObj (PageDirectory pd)))"
   "typ_at (AArch APDPointerTable) p s \<longleftrightarrow> (\<exists>pdpt. kheap s p = Some (ArchObj (PDPointerTable pdpt)))"
   "typ_at (AArch APageMapL4) p s \<longleftrightarrow> (\<exists>pm. kheap s p = Some (ArchObj (PageMapL4 pm)))"
-  "typ_at (AArch (AIntData sz)) p s \<longleftrightarrow> (kheap s p = Some (ArchObj (DataPage sz)))"
+  "typ_at (AArch (AUserData sz)) p s \<longleftrightarrow> (kheap s p = Some (ArchObj (DataPage False sz)))"
+  "typ_at (AArch (ADeviceData sz)) p s \<longleftrightarrow> (kheap s p = Some (ArchObj (DataPage True sz)))"
   apply (auto simp add: obj_at_def)
   apply (simp_all add: a_type_def
                 split: split_if_asm kernel_object.splits arch_kernel_obj.splits)
@@ -1274,30 +1326,24 @@ lemma shows
    aa_type_APageTableE:
   "\<lbrakk>a_type ko = AArch APageTable; (\<And>pt. ko = ArchObj (PageTable pt) \<Longrightarrow> R)\<rbrakk>
    \<Longrightarrow> R" and
-   aa_type_AIntDataE:
-  "\<lbrakk>a_type ko = AArch (AIntData sz); ko = ArchObj (DataPage sz) \<Longrightarrow> R\<rbrakk> \<Longrightarrow> R"
+   aa_type_AUserDataE:
+  "\<lbrakk>a_type ko = AArch (AUserData sz); ko = ArchObj (DataPage False sz) \<Longrightarrow> R\<rbrakk> \<Longrightarrow> R"
+  and
+   aa_type_ADeviceDataE:
+  "\<lbrakk>a_type ko = AArch (ADeviceData sz); ko = ArchObj (DataPage True sz) \<Longrightarrow> R\<rbrakk> \<Longrightarrow> R"
   by (rule kernel_object_exhaust[of ko]; clarsimp simp add: a_type_simps split: split_if_asm)+
 
 lemmas aa_type_elims[elim!] =
-   aa_type_AASIDPoolE aa_type_APageDirectoryE aa_type_APageTableE aa_type_AIntDataE
-   aa_type_APDPointerTableE aa_type_APageMapL4E
+   aa_type_AASIDPoolE aa_type_AUserDataE aa_type_ADeviceDataE
+   aa_type_APageDirectoryE aa_type_APageTableE aa_type_APDPointerTableE aa_type_APageMapL4E
 
 lemma valid_arch_obj_pspaceI:
   "\<lbrakk> valid_arch_obj obj s; kheap s = kheap s' \<rbrakk> \<Longrightarrow> valid_arch_obj obj s'"
-  apply (cases obj, simp_all)
-      apply (simp add: obj_at_def)
-     apply (erule allEI)
-     apply (rename_tac "fun" x)
-     apply (case_tac "fun x", simp_all add: obj_at_def)
-    apply (erule allEI)
-    apply (rename_tac "fun" x)
-    apply (case_tac "fun x", simp_all add: obj_at_def)
-   apply (erule allEI)
-   apply (rename_tac "fun" x)
-   apply (case_tac "fun x", simp_all add: obj_at_def)
-  apply (erule ballEI)
-  apply (rename_tac "fun" x)
-  apply (case_tac "fun x", simp_all add: obj_at_def)
+  apply (cases obj, simp_all add: obj_at_def)
+     apply (erule allEI ballEI,
+            rename_tac "fun" x,
+            case_tac "fun x",
+            simp_all add: obj_at_def data_at_def)+
   done
 
 lemmas  pageBitsForSize_simps[simp] =
@@ -1340,6 +1386,10 @@ lemma in_user_frame_update[iff]:
   "in_user_frame p (f s) = in_user_frame p s"
   by (simp add: in_user_frame_def pspace)
 
+lemma in_device_frame_update[iff]:
+  "in_device_frame p (f s) = in_device_frame p s"
+  by (simp add: in_device_frame_def obj_at_def pspace)
+
 lemma obj_at_update [iff]:
   "obj_at P p (f s) = obj_at P p s"
   by (fastforce intro: obj_at_pspaceI simp: pspace)
@@ -1365,20 +1415,20 @@ lemma valid_global_pdpts_update [iff]:
 
 lemma valid_pte_update [iff]:
   "valid_pte pte (f s) = valid_pte pte s"
-  by (cases pte) auto
+  by (cases pte) (auto simp: data_at_def)
 
 lemma valid_pde_update [iff]:
   "valid_pde pde (f s) = valid_pde pde s"
-  by (cases pde) auto
+  by (cases pde) (auto simp: data_at_def)
   
 lemma valid_pdpte_update [iff]:
-  "valid_pdpte pte (f s) = valid_pdpte pte s"
-  by (cases pte) auto
+  "valid_pdpte pdpte (f s) = valid_pdpte pdpte s"
+  by (cases pdpte) (auto simp: data_at_def)
 
 lemma valid_pml4e_update [iff]:
-  "valid_pml4e pte (f s) = valid_pml4e pte s"
-  by (cases pte) auto
-  
+  "valid_pml4e pml4e (f s) = valid_pml4e pml4e s"
+  by (cases pml4e) auto
+
 lemma valid_arch_obj_update [iff]:
   "valid_arch_obj ao (f s) = valid_arch_obj ao s"
   by (cases ao) auto
@@ -1520,8 +1570,8 @@ lemma valid_arch_state_lift:
 
 lemma aobj_at_default_arch_cap_valid:
   assumes "ty \<noteq> ASIDPoolObj"
-  assumes "ko_at (ArchObj (default_arch_object ty us)) x s"
-  shows "valid_arch_cap (arch_default_cap ty x us) s"
+  assumes "ko_at (ArchObj (default_arch_object ty dev us)) x s"
+  shows "valid_arch_cap (arch_default_cap ty x us dev) s"
   using assms
   by (auto elim!: obj_at_weakenE
         simp add: arch_default_cap_def valid_arch_cap_def default_arch_object_def
@@ -1530,7 +1580,7 @@ lemma aobj_at_default_arch_cap_valid:
            split: apiobject_type.splits aobject_type.splits option.splits)
 
 lemma aobj_ref_default:
-  "aobj_ref (arch_default_cap x6 x us) = Some x"
+  "aobj_ref (arch_default_cap x6 x us dev) = Some x"
   by (auto simp add: arch_default_cap_def split: aobject_type.splits)
 
 lemma valid_pml4e_lift:
@@ -1541,17 +1591,17 @@ lemma valid_pml4e_lift:
 lemma valid_pdpte_lift:
   assumes x: "\<And>T p. \<lbrace>typ_at (AArch T) p\<rbrace> f \<lbrace>\<lambda>rv. typ_at (AArch T) p\<rbrace>"
   shows "\<lbrace>\<lambda>s. valid_pdpte pdpte s\<rbrace> f \<lbrace>\<lambda>rv s. valid_pdpte pdpte s\<rbrace>"
-  by (cases pdpte) (simp | wp x)+
+  by (cases pdpte) (simp add: data_at_def | wp hoare_vcg_disj_lift x)+
   
 lemma valid_pde_lift:
   assumes x: "\<And>T p. \<lbrace>typ_at (AArch T) p\<rbrace> f \<lbrace>\<lambda>rv. typ_at (AArch T) p\<rbrace>"
   shows "\<lbrace>\<lambda>s. valid_pde pde s\<rbrace> f \<lbrace>\<lambda>rv s. valid_pde pde s\<rbrace>"
-  by (cases pde) (simp | wp x)+
+  by (cases pde) (simp add: data_at_def | wp hoare_vcg_disj_lift x)+
 
 lemma valid_pte_lift:
   assumes x: "\<And>T p. \<lbrace>typ_at (AArch T) p\<rbrace> f \<lbrace>\<lambda>rv. typ_at (AArch T) p\<rbrace>"
   shows "\<lbrace>\<lambda>s. valid_pte pte s\<rbrace> f \<lbrace>\<lambda>rv s. valid_pte pte s\<rbrace>"
-  by (cases pte) (simp | wp x)+
+  by (cases pte) (simp add: data_at_def | wp hoare_vcg_disj_lift x)+
 
 lemma pdpte_at_atyp:
   assumes x: "\<And>p T. \<lbrace>typ_at (AArch T) p\<rbrace> f \<lbrace>\<lambda>rv. typ_at (AArch T) p\<rbrace>"
@@ -2339,10 +2389,10 @@ proof -
     apply (erule converse_rtranclE)
      apply clarsimp
      apply (erule (12) 5)
-    apply (clarsimp simp:vs_refs_pages_def graph_of_def obj_at_def
-                          pte_ref_pages_def
-                   dest!: vs_lookup_pages1D
-                   split: pte.splits)
+    apply (auto simp: vs_refs_pages_def graph_of_def obj_at_def
+                      pte_ref_pages_def data_at_def
+               dest!: vs_lookup_pages1D
+               split: pte.splits)
     done
 qed
 
@@ -2528,17 +2578,17 @@ by (simp add: addrFromPPtr_def ptrFromPAddr_def)
 lemma valid_pte_lift2:
   assumes x: "\<And>T p. \<lbrace>Q and typ_at (AArch T) p\<rbrace> f \<lbrace>\<lambda>rv. typ_at (AArch T) p\<rbrace>"
   shows "\<lbrace>\<lambda>s. Q s \<and> valid_pte pte s\<rbrace> f \<lbrace>\<lambda>rv s. valid_pte pte s\<rbrace>"
-  by (cases pte) (simp | wp x)+
+  by (cases pte) (simp add: data_at_def | wp hoare_vcg_disj_lift x)+
 
 lemma valid_pde_lift2:
   assumes x: "\<And>T p. \<lbrace>Q and typ_at (AArch T) p\<rbrace> f \<lbrace>\<lambda>rv. typ_at (AArch T) p\<rbrace>"
   shows "\<lbrace>\<lambda>s. Q s \<and> valid_pde pde s\<rbrace> f \<lbrace>\<lambda>rv s. valid_pde pde s\<rbrace>"
-  by (cases pde) (simp | wp x)+
+  by (cases pde) (simp add: data_at_def | wp hoare_vcg_disj_lift x)+
 
 lemma valid_pdpte_lift2:
   assumes x: "\<And>T p. \<lbrace>Q and typ_at (AArch T) p\<rbrace> f \<lbrace>\<lambda>rv. typ_at (AArch T) p\<rbrace>"
   shows "\<lbrace>\<lambda>s. Q s \<and> valid_pdpte pde s\<rbrace> f \<lbrace>\<lambda>rv s. valid_pdpte pde s\<rbrace>"
-  by (cases pde) (simp | wp x)+
+  by (cases pde) (simp add: data_at_def | wp hoare_vcg_disj_lift x)+
   
 lemma valid_pml4e_lift2:
   assumes x: "\<And>T p. \<lbrace>Q and typ_at (AArch T) p\<rbrace> f \<lbrace>\<lambda>rv. typ_at (AArch T) p\<rbrace>"
@@ -2725,7 +2775,7 @@ lemmas cap_asid_simps [simp] =
 
 lemma in_user_frame_def:
   "in_user_frame p \<equiv> \<lambda>s.
-   \<exists>sz. typ_at (AArch (AIntData sz)) (p && ~~ mask (pageBitsForSize sz)) s"
+   \<exists>sz. typ_at (AArch (AUserData sz)) (p && ~~ mask (pageBitsForSize sz)) s"
   apply (rule eq_reflection, rule ext)
   apply (simp add: in_user_frame_def obj_at_def)
   apply (rule_tac f=Ex in arg_cong)
@@ -2741,12 +2791,12 @@ lemma in_user_frame_lift:
  by (wp hoare_vcg_ex_lift typ_at)
 
 lemma wellformed_arch_default: 
-  "wellformed_arch_obj (default_arch_object aobject_type us)"
+  "wellformed_arch_obj (default_arch_object aobject_type dev us)"
   unfolding wellformed_arch_obj_def default_arch_object_def
   by (cases aobject_type; simp)
 
 lemma valid_arch_obj_default': 
-  "valid_arch_obj (default_arch_object aobject_type us) s"
+  "valid_arch_obj (default_arch_object aobject_type dev us) s"
   unfolding default_arch_object_def
   by (cases aobject_type; simp)
 
