proof/invariant-abstract/X64/ArchCSpaceInv_AI.thy
@@ -31,7 +31,8 @@ lemma replace_cap_invs:
              set_cap_caps_of_state2 set_cap_idle
              replace_cap_ifunsafe valid_irq_node_typ
              set_cap_typ_at set_cap_irq_handlers
-             set_cap_valid_arch_caps)
+             set_cap_valid_arch_caps
+             set_cap_cap_refs_respects_device_region_replaceable)
   apply (clarsimp simp: valid_pspace_def cte_wp_at_caps_of_state
                         replaceable_def)
   apply (rule conjI)
@@ -107,8 +108,7 @@ lemma replace_cap_invs:
    apply (clarsimp simp: valid_table_capsD[OF caps_of_state_cteD]
                     valid_arch_caps_def unique_table_refs_no_cap_asidE)
   apply simp
-  apply (rule Ball_emptyI)
-  apply (simp add: obj_irq_refs_subset)
+  apply (rule Ball_emptyI, simp add: obj_irq_refs_subset)
   done
 
 end
