spec/abstract/X64/ArchRetype_A.thy
@@ -32,25 +32,25 @@ text {* Create 4096-byte frame objects that can be mapped into memory. These mus
 cleared to prevent past contents being revealed. *}
 
 definition
-  create_word_objects :: "machine_word \<Rightarrow> nat \<Rightarrow> nat \<Rightarrow> (unit,'z::state_ext) s_monad" where
-  "create_word_objects ptr numObjects sz \<equiv>
+  create_word_objects :: "machine_word \<Rightarrow> nat \<Rightarrow> nat \<Rightarrow> bool \<Rightarrow> (unit,'z::state_ext) s_monad" where
+  "create_word_objects ptr numObjects sz is_device \<equiv>
   do
     byteLength \<leftarrow> return $ numObjects * 2 ^ sz;
     reserve_region ptr byteLength True;
     rst \<leftarrow>  return (map (\<lambda> n. (ptr + (n << sz))) [0  .e.  (of_nat numObjects) - 1]);
-    do_machine_op $ mapM_x (\<lambda>x. clearMemory x (2 ^ sz)) rst
+    unless is_device $ do_machine_op $ mapM_x (\<lambda>x. clearMemory x (2 ^ sz)) rst
  od"
 
 text {* Initialise architecture-specific objects. *}
 
 definition
-  init_arch_objects :: "apiobject_type \<Rightarrow> obj_ref \<Rightarrow> nat \<Rightarrow> nat \<Rightarrow> obj_ref list
+  init_arch_objects :: "apiobject_type \<Rightarrow> obj_ref \<Rightarrow> nat \<Rightarrow> nat \<Rightarrow> obj_ref list \<Rightarrow> bool
    \<Rightarrow> (unit,'z::state_ext) s_monad"
 where
-  "init_arch_objects new_type ptr num_objects obj_sz refs \<equiv> case new_type of
-    ArchObject SmallPageObj \<Rightarrow> create_word_objects ptr num_objects 12
-  | ArchObject LargePageObj \<Rightarrow> create_word_objects ptr num_objects 16
-  | ArchObject HugePageObj \<Rightarrow> create_word_objects ptr num_objects 20
+  "init_arch_objects new_type ptr num_objects obj_sz refs is_device \<equiv> case new_type of
+    ArchObject SmallPageObj \<Rightarrow> create_word_objects ptr num_objects 12 is_device
+  | ArchObject LargePageObj \<Rightarrow> create_word_objects ptr num_objects 16 is_device
+  | ArchObject HugePageObj \<Rightarrow> create_word_objects ptr num_objects 20 is_device
   | ArchObject PageTableObj \<Rightarrow> return ()
   | ArchObject PageDirectoryObj \<Rightarrow> return ()
   | ArchObject PDPTObj \<Rightarrow> mapM_x copy_global_mappings refs
